some more steps on the way to using symb_prop_transfer_thm for incr example

examples/riscv/incr/incr_propScript.sml
@@ -17,6 +17,8 @@ open bir_wp_interfaceLib;
 
 open tutorial_smtSupportLib;
 
+open bir_symbTheory birs_auxTheory;
+open HolBACoreSimps;
 open bir_program_transfTheory;
 
 open total_program_logicTheory;
@@ -32,6 +34,8 @@ open incrTheory;
 open incr_symb_execTheory;
 
 val _ = new_theory "incr_prop";
+
+(* ------ *)
 
 Definition riscv_incr_pre_def:
  riscv_incr_pre (m : riscv_state) = T (* FIXME *)
@@ -49,23 +53,142 @@ Definition bir_incr_post_def:
  bir_incr_post : bir_exp_t = bir_exp_true (* FIXME *)
 End
 
-(*
-Theorem abstract_jgmt_rel_incr[local]:
- abstract_jgmt_rel (bir_ts bprog) (BL_Address (Imm64 0w)) {BL_Address (Imm64 8w)}
-  (\st. bir_exec_to_labels_triple_precond st pre bir_incr_prog)
-  (\st st'. bir_exec_to_labels_triple_postcond st' post bprog)
+(* ------ *)
+
+val (sys_i, L_s, Pi_f) = (symb_sound_struct_get_sysLPi_fun o concl) incr_symb_analysis_thm;
+
+Definition incr_analysis_L_def:
+ incr_analysis_L = ^(L_s)
+End
+
+val birs_state_init_lbl = ``<|bpc_label := BL_Address (Imm64 0w); bpc_index := 0|>``;
+val birs_state_end_lbl = (snd o dest_eq o concl o EVAL) ``bir_block_pc (BL_Address (Imm64 8w))``;
+
+Definition bprecond_def:
+  bprecond = bir_exp_true
+End
+
+val bprecond = (fst o dest_eq o concl) bprecond_def;
+
+Definition bsysprecond_def:
+  bsysprecond = FST (THE (birs_eval_exp ^bprecond (bir_senv_GEN_list birenvtyl_riscv)))
+End
+
+Theorem bprecond_birs_eval_exp_thm = (computeLib.RESTR_EVAL_CONV [``birs_eval_exp``] THENC
+   birs_stepLib.birs_eval_exp_CONV)
+     ``birs_eval_exp bprecond (bir_senv_GEN_list birenvtyl_riscv)``
+
+Theorem bsysprecond_thm =
+ (REWRITE_CONV [bsysprecond_def, birs_eval_exp_ALT_thm, bprecond_birs_eval_exp_thm] THENC EVAL) ``bsysprecond``
+
+Theorem bprecond_birs_eval_exp_thm2 = REWRITE_CONV [bprecond_birs_eval_exp_thm, GSYM bsysprecond_thm] ``birs_eval_exp bprecond (bir_senv_GEN_list birenvtyl_riscv)``
+
+val bsysprecond = (fst o dest_eq o concl) bsysprecond_def;
+
+val birs_state_init_pre = ``<|
+  bsst_pc       := ^birs_state_init_lbl;
+  bsst_environ  := bir_senv_GEN_list birenvtyl_riscv;
+  bsst_status   := BST_Running;
+  bsst_pcond    := ^bsysprecond
+|>``;
+
+val birs_state_ss = rewrites (type_rws ``:birs_state_t``);
+val birs_state_init_pre_EQ_thm =
+ REWRITE_RULE [] ((REWRITE_CONV [bsysprecond_thm] THENC
+  SIMP_CONV (std_ss++birs_state_ss++holBACore_ss) [] THENC
+  EVAL)
+  ``^((snd o dest_comb) sys_i) = ^birs_state_init_pre``);
+
+val incr_analysis_thm =
+  REWRITE_RULE [birs_state_init_pre_EQ_thm] incr_symb_analysis_thm;
+
+Theorem birenvtyl_riscv_EVAL_thm =
+ (REWRITE_CONV [birenvtyl_riscv_def, riscv_vars_def,
+   bir_lifting_machinesTheory.riscv_bmr_vars_EVAL,
+   bir_lifting_machinesTheory.riscv_bmr_temp_vars_EVAL] THENC EVAL) ``birenvtyl_riscv``
+
+val birs_state_thm = REWRITE_CONV [birenvtyl_riscv_EVAL_thm] birs_state_init_pre;
+
+(* ------ *)
+
+(* now the transfer *)
+
+val bprog_tm = (fst o dest_eq o concl) bir_incr_prog_def;
+
+val birs_symb_symbols_f_sound_prog_thm =
+  (SPEC (inst [Type`:'observation_type` |-> Type.alpha] bprog_tm) bir_symb_soundTheory.birs_symb_symbols_f_sound_thm);
+
+val birs_prop_transfer_thm =
+  (MATCH_MP symb_prop_transferTheory.symb_prop_transfer_thm birs_symb_symbols_f_sound_prog_thm);
+
+Definition bprog_P_def:
+  bprog_P ((SymbConcSt pc st status):(bir_programcounter_t, string, bir_val_t, bir_status_t) symb_concst_t) =
+      (status = BST_Running /\
+       pc.bpc_index = 0 /\
+       bir_envty_list birenvtyl_riscv st /\
+       bir_eval_exp ^bprecond (BEnv st) = SOME bir_val_true)
+End
+
+(* translate the property to BIR state property *)
+Theorem bprog_P_thm:
+  !bs.
+  bprog_P (birs_symb_to_concst bs) =
+      (bs.bst_status = BST_Running /\
+       bs.bst_pc.bpc_index = 0 /\
+       bir_envty_list_b birenvtyl_riscv bs.bst_environ /\
+       bir_eval_exp ^bprecond bs.bst_environ = SOME bir_val_true)
 Proof
- (* reasoning using symbolic execution goes here *)
+ REPEAT STRIP_TAC >>
+  FULL_SIMP_TAC (std_ss) [birs_symb_to_concst_def, bprog_P_def, bir_envty_list_b_thm, bir_BEnv_lookup_EQ_thm]
+QED
+
+Definition bprog_Q_def:
+  bprog_Q
+     ((SymbConcSt pc1 st1 status1):(bir_programcounter_t, string, bir_val_t, bir_status_t) symb_concst_t)
+     ((SymbConcSt pc2 st2 status2):(bir_programcounter_t, string, bir_val_t, bir_status_t) symb_concst_t)
+    =
+     (
+       (pc2 = ^birs_state_end_lbl)
+       /\
+       (status2 = BST_Running)
+     )
+End
+
+Theorem bprog_Q_thm:
+  !bs1 bs2.
+  bprog_Q (birs_symb_to_concst bs1) (birs_symb_to_concst bs2) =
+    (
+      (bs2.bst_pc = ^birs_state_end_lbl)
+      /\
+      (bs2.bst_status = BST_Running)
+    )
+Proof
+FULL_SIMP_TAC (std_ss) [birs_symb_to_concst_def, bprog_Q_def]
+QED
+
+Theorem abstract_jgmt_rel_incr[local]:
+ abstract_jgmt_rel (bir_ts bir_incr_prog) (BL_Address (Imm64 0w)) {BL_Address (Imm64 8w)}
+  (\st. bir_exec_to_labels_triple_precond st bir_incr_pre bir_incr_prog)
+  (\st st'. bir_exec_to_labels_triple_postcond st' (\l. if l = BL_Address (Imm64 8w) then bir_incr_post else bir_exp_false) bir_incr_prog)
+Proof
+ (* reasoning via symb_prop_transfer_thm goes here *)
  cheat
 QED
-*)
 
 Theorem bir_cont_incr[local]:
  bir_cont bir_incr_prog bir_exp_true (BL_Address (Imm64 0w))
   {BL_Address (Imm64 8w)} {} bir_incr_pre
   (\l. if l = BL_Address (Imm64 8w) then bir_incr_post else bir_exp_false)
 Proof
- cheat
+ `{BL_Address (Imm64 8w)} <> {}` by fs [] >>
+ MP_TAC (Q.SPECL [`bir_incr_prog`,
+  `BL_Address (Imm64 0w)`,
+  `{BL_Address (Imm64 8w)}`,
+  `bir_incr_pre`,
+  `\l. if l = BL_Address (Imm64 8w) then bir_incr_post else bir_exp_false`
+ ] abstract_jgmt_rel_bir_cont) >>
+ rw [] >>
+ METIS_TAC [abstract_jgmt_rel_incr]
 QED
 
 (* TODO: RISC-V backlifting *)
